Vegas/Machine.lean
@@ -45,6 +45,7 @@ import Vegas.Machine.Contract.ClassicalEVMIR
 import Vegas.Machine.Contract.EVMAssembly
 import Vegas.Machine.Contract.EVMLocalAssembly
 import Vegas.Machine.Contract.EVMDeployment
+import Vegas.Machine.Contract.EVMExecution
 import Vegas.Machine.Contract.Imperative
 import Vegas.Machine.Contract.ClassicalEVMCodegen
 import Vegas.Machine.Contract.SimpleEVMExpr
